rocq-osiris/theories/logic/list_init.v
@@ -1,0 +1,179 @@
+From stdpp Require Import list.
+
+(** [init_segment i n f] is a list of length [n] whose elements are [f(i)],
+    [f(i+1)], etc., up to [f(i+n-1)]. *)
+Fixpoint init_segment {A} (i : nat) (n : nat) (f : nat → A) : list A :=
+  match n with 0 => [] | S n => f i :: init_segment (i + 1) n f end.
+
+(** [init n f] is a list of length [n] whose elements are [f(0)],
+    [f(1)], etc., up to [f(n-1)]. *)
+Definition init {A} (n : nat) (f : nat → A) : list A :=
+  init_segment 0 n f.
+
+(** ** Properties of [init_segment] and [init] *)
+
+Section Init.
+Context {A : Type}.
+Implicit Types xs : list A.
+Implicit Types f : nat → A.
+
+(* Interaction with [length]. *)
+
+Lemma length_init_segment i n f : length (init_segment i n f) = n.
+Proof.
+  revert i. induction n; simpl; congruence.
+Qed.
+
+Lemma length_init n f : length (init n f) = n.
+Proof. unfold init. apply length_init_segment. Qed.
+
+(* Interaction with [lookup]. *)
+
+Lemma lookup_init_segment_lt i n f k :
+  k < n →
+  init_segment i n f !! k = Some (f (i + k)).
+Proof.
+  revert i k. induction n; simpl; intros; [ lia |].
+  rewrite lookup_cons.
+  destruct k as [| k]; try rewrite IHn by lia;
+  do 2 f_equal; lia.
+Qed.
+
+Lemma lookup_init_segment_ge i n f k :
+  n ≤ k →
+  init_segment i n f !! k = None.
+Proof.
+  revert i k. induction n; simpl; intros; [ eauto |].
+  rewrite lookup_cons.
+  destruct k as [| k]; try rewrite IHn by lia;
+  eauto with lia.
+Qed.
+
+Lemma lookup_init_segment i n f k :
+  init_segment i n f !! k =
+    if decide (k < n) then Some (f (i + k)) else None.
+Proof.
+  case_decide;
+  eauto using lookup_init_segment_lt, lookup_init_segment_ge with lia.
+Qed.
+
+Lemma lookup_init_lt n f k :
+  k < n →
+  init n f !! k = Some (f k).
+Proof.
+  unfold init. eauto using lookup_init_segment_lt.
+Qed.
+
+Lemma lookup_init_ge n f k :
+  n ≤ k →
+  init n f !! k = None.
+Proof.
+  unfold init. eauto using lookup_init_segment_ge.
+Qed.
+
+Lemma lookup_init n f k :
+  init n f !! k =
+    if decide (k < n) then Some (f k) else None.
+Proof.
+  case_decide; eauto using lookup_init_lt, lookup_init_ge with lia.
+Qed.
+
+(* Interaction with [lookup_total]. *)
+
+Section LookupTotal.
+Context `{Inhabited A}.
+
+Local Ltac translate lemma :=
+  intros; rewrite !list_lookup_total_alt;
+  rewrite lemma by lia; repeat case_decide; eauto.
+
+Lemma lookup_total_init_segment_lt i n f k :
+  k < n →
+  init_segment i n f !!! k = f (i + k).
+Proof.
+  translate lookup_init_segment_lt.
+Qed.
+
+Lemma lookup_total_init_segment_ge i n f k :
+  n ≤ k →
+  init_segment i n f !!! k = inhabitant.
+Proof.
+  translate lookup_init_segment_ge.
+Qed.
+
+Lemma lookup_total_init_segment i n f k :
+  init_segment i n f !!! k =
+    if decide (k < n) then f (i + k) else inhabitant.
+Proof.
+  translate lookup_init_segment.
+Qed.
+
+Lemma lookup_total_init_lt n f k :
+  k < n →
+  init n f !!! k = f k.
+Proof.
+  translate lookup_init_lt.
+Qed.
+
+Lemma lookup_total_init_ge n f k :
+  n ≤ k →
+  init n f !!! k = inhabitant.
+Proof.
+  translate lookup_init_ge.
+Qed.
+
+Lemma lookup_total_init n f k :
+  init n f !!! k =
+    if decide (k < n) then f k else inhabitant.
+Proof.
+  translate lookup_init.
+Qed.
+
+End LookupTotal.
+
+(* Interaction of [take] and [init]. *)
+
+Lemma take_init n m f :
+  take n (init m f) = init (n `min` m) f.
+Proof.
+  eapply list_eq_same_length.
+  + rewrite length_init. eauto.
+  + rewrite length_take, length_init. eauto.
+  + intros i x y ?.
+    rewrite lookup_take, !lookup_init.
+    repeat case_decide; congruence.
+Qed.
+
+(* Interaction of [drop] and [init]. *)
+
+Lemma drop_init n m f :
+  drop n (init m f) = init (m - n) (λ i, f (n + i)).
+Proof.
+  eapply list_eq_same_length.
+  + rewrite length_init. eauto.
+  + rewrite length_drop, length_init. eauto.
+  + intros i x y ?.
+    rewrite lookup_drop, !lookup_init.
+    repeat case_decide; congruence.
+Qed.
+
+(* Extension of [init] with one more element. *)
+
+Lemma init_segment_app_singleton i n f x :
+  f (i + n) = x →
+  init_segment i n f ++ [x] = init_segment i (n + 1) f.
+Proof.
+  revert i.
+  induction n as [| n]; simpl; intros; subst x; do 2 f_equal.
+  + lia.
+  + rewrite IHn by (f_equal; lia). eauto.
+Qed.
+
+Lemma init_app_singleton n f x :
+  f n = x →
+  init n f ++ [x] = init (n + 1) f.
+Proof.
+  intros. subst x. unfold init. eapply init_segment_app_singleton. eauto.
+Qed.
+
+End Init.
